Back to edom ae = edom ce

Launchbury/CardinalityEtaExpand.thy
@@ -49,18 +49,18 @@ begin
   definition anal_env :: "(exp \<Rightarrow> 'a::cpo \<rightarrow> 'b::pcpo) \<Rightarrow> heap \<Rightarrow> (var \<Rightarrow> 'a\<^sub>\<bottom>) \<rightarrow> (var \<Rightarrow> 'b)"
     where "anal_env f \<Gamma> = (\<Lambda> e. (\<lambda> x . fup\<cdot>(f (the (map_of \<Gamma> x)))\<cdot>(e x)))"
 
+
   inductive consistent :: "tstate \<Rightarrow> conf \<Rightarrow> bool" where
     consistentI[intro!]: 
-    "edom ae \<subseteq> domA \<Gamma> \<union> upds S
-    \<Longrightarrow> edom ce \<subseteq> domA \<Gamma> \<union> upds S
+    "edom ce \<subseteq> domA \<Gamma> \<union> upds S
     \<Longrightarrow> heap_upds_ok (\<Gamma>, S)
-    \<Longrightarrow> edom ce \<subseteq> edom ae
+    \<Longrightarrow> edom ae = edom ce
     \<Longrightarrow> Astack (restr_stack (edom ce) S) \<sqsubseteq> a
     \<Longrightarrow> prognosis ae a (\<Gamma>, e, S) \<sqsubseteq> ce
-    \<Longrightarrow> ABinds (restrictA (edom ce) \<Gamma>)\<cdot>ae \<squnion> Aexp e\<cdot>a \<sqsubseteq> ae
+    \<Longrightarrow> (ABinds \<Gamma>\<cdot>ae \<squnion> Aexp e\<cdot>a) f|` edom ce \<sqsubseteq> ae
     \<Longrightarrow> (\<And> x. x \<in> thunks \<Gamma> \<Longrightarrow> many \<sqsubseteq> ce x \<Longrightarrow> ae x = up\<cdot>0)
-    \<Longrightarrow> const_on ae (ap S) (up\<cdot>0)
-    \<Longrightarrow> const_on ae (upds (restr_stack (edom ce) S)) (up\<cdot>0)
+    \<Longrightarrow> const_on ae (ap S \<inter> edom ce) (up\<cdot>0)
+    \<Longrightarrow> const_on ae (upds S \<inter> edom ce) (up\<cdot>0)
     \<Longrightarrow> consistent (ae, ce, a) (\<Gamma>, e, S)"  
   inductive_cases consistentE[elim!]: "consistent (ae, ce, a) (\<Gamma>, e, S)"
 
@@ -79,7 +79,7 @@ begin
     show ?thesis
       by (auto simp add: edom_empty_iff_bot)
   qed
-  
+
   lemma foo:
     fixes c c' R 
     assumes "c \<Rightarrow>\<^sup>* c'" and "\<not> boring_step c'" and "consistent (ae,ce,a) c"
@@ -89,7 +89,7 @@ begin
   case (app\<^sub>1 \<Gamma> e x S)
     have "prognosis ae (inc\<cdot>a) (\<Gamma>, e, Arg x # S) \<sqsubseteq> prognosis ae a (\<Gamma>, App e x, S)" by (rule prognosis_App)
     with app\<^sub>1 have "consistent (ae, ce, inc\<cdot>a) (\<Gamma>, e, Arg x # S)"
-      by (auto simp add: join_below_iff  dest!: below_trans[OF Aexp_App] elim: below_trans)
+      by (cases "x \<in> edom ce")  (auto simp add: join_below_iff env_restr_join dest!: below_trans[OF env_restr_mono[OF Aexp_App]] elim: below_trans)
     moreover
     have "conf_transform (ae, ce, a) (\<Gamma>, App e x, S) \<Rightarrow>\<^sub>G conf_transform (ae, ce, inc\<cdot>a) (\<Gamma>, e, Arg x # S)"
       by simp rule
@@ -101,16 +101,17 @@ begin
        by (rule prognosis_subst_Lam)
     moreover
     {
-    have "Aexp (e[y::=x])\<cdot>(pred\<cdot>a) \<sqsubseteq> env_delete y ((Aexp e)\<cdot>(pred\<cdot>a)) \<squnion> esing x\<cdot>(up\<cdot>0)" by (rule Aexp_subst)
+    have "Aexp (e[y::=x])\<cdot>(pred\<cdot>a) f|` edom ce  \<sqsubseteq> (env_delete y ((Aexp e)\<cdot>(pred\<cdot>a)) \<squnion> esing x\<cdot>(up\<cdot>0)) f|` edom ce" by (rule env_restr_mono[OF Aexp_subst])
+    also have "\<dots> =  env_delete y ((Aexp e)\<cdot>(pred\<cdot>a))  f|` edom ce \<squnion> esing x\<cdot>(up\<cdot>0)  f|` edom ce" by (simp add: env_restr_join)
     also have "env_delete y ((Aexp e)\<cdot>(pred\<cdot>a)) \<sqsubseteq> Aexp (Lam [y]. e)\<cdot>a" by (rule Aexp_Lam)
-    also have "\<dots> \<sqsubseteq> ae" using app\<^sub>2 by (auto simp add: join_below_iff)
-    also have "esing x\<cdot>(up\<cdot>0) \<sqsubseteq> ae" using app\<^sub>2 by auto
+    also have "\<dots> f|` edom ce \<sqsubseteq> ae" using app\<^sub>2 by (auto simp add: join_below_iff env_restr_join)
+    also have "esing x\<cdot>(up\<cdot>0) f|` edom ce  \<sqsubseteq> ae" using app\<^sub>2 by (cases "x\<in>edom ce") (auto simp add: env_restr_join)
     also have "ae \<squnion> ae = ae" by simp
-    finally  have "Aexp (e[y::=x])\<cdot>(pred\<cdot>a) \<sqsubseteq> ae" by this simp_all
+    finally  have "Aexp (e[y::=x])\<cdot>(pred\<cdot>a) f|` edom ce \<sqsubseteq> ae" by this simp_all
     }
     ultimately
     have "consistent (ae, ce, pred\<cdot>a) (\<Gamma>, e[y::=x], S)" using app\<^sub>2
-      by (auto elim: below_trans edom_mono  simp add: join_below_iff)
+      by (auto elim: below_trans edom_mono  simp add: join_below_iff env_restr_join)
     moreover
     have "conf_transform (ae, ce, a) (\<Gamma>, Lam [y]. e, Arg x # S) \<Rightarrow>\<^sub>G conf_transform (ae, ce, pred \<cdot> a) (\<Gamma>, e[y::=x], S)" by (simp add: subst_transform[symmetric]) rule
     ultimately
@@ -120,26 +121,26 @@ begin
     hence "x \<in> thunks \<Gamma>" by auto
     hence [simp]: "x \<in> domA \<Gamma>" by (rule set_mp[OF thunks_domA])
     hence "x \<notin> upds S" using thunk by (auto elim!: heap_upds_okE)
-  
-    from thunk have "Aexp (Var x)\<cdot>a \<sqsubseteq> ae" by (auto simp add: join_below_iff)
-    from below_trans[OF Aexp_Var fun_belowD[OF this] ]
-    have "up\<cdot>a \<sqsubseteq> ae x".    
-    then obtain u where "ae x = up\<cdot>u" and "a \<sqsubseteq> u" by (cases "ae x") auto
-    hence [simp]: "x \<in> edom ae" by (simp add: edom_def)
 
     from thunk have "prognosis ae a (\<Gamma>, Var x, S) \<sqsubseteq> ce" by auto
     from below_trans[OF prognosis_called fun_belowD[OF this] ]
     have [simp]: "x \<in> edom ce" by (auto simp add: edom_def)
+  
+    from thunk
+    have "Aexp (Var x)\<cdot>a  f|` edom ce \<sqsubseteq> ae" by (auto simp add: join_below_iff env_restr_join)
+    from fun_belowD[where x = x, OF this] 
+    have "(Aexp (Var x)\<cdot>a) x \<sqsubseteq> ae x" by simp
+    from below_trans[OF  Aexp_Var this]
+    have "up\<cdot>a \<sqsubseteq> ae x".    
+    then obtain u where "ae x = up\<cdot>u" and "a \<sqsubseteq> u" by (cases "ae x") auto
+    hence [simp]: "x \<in> edom ae" by (simp add: edom_def)
 
     have "Astack (restr_stack (edom ce) S) \<sqsubseteq> u" using thunk `a \<sqsubseteq> u` by (auto elim: below_trans)
   
-    from `map_of \<Gamma> x = Some e`
-    have "map_of (restrictA (edom ce) \<Gamma>) x = Some e" by simp
-    from Abinds_reorder1[OF this] `ae x = up\<cdot>u`
-    have "ABinds (delete x (restrictA (edom ce) \<Gamma>))\<cdot>ae \<squnion> Aexp e\<cdot>u = ABinds (restrictA (edom ce) \<Gamma>)\<cdot>ae" by (auto intro: join_comm)
-    also have "\<dots> \<sqsubseteq> ae" using thunk by (auto simp add: join_below_iff)
-    finally have "ABinds (delete x (restrictA (edom ce) \<Gamma>))\<cdot>ae \<squnion> Aexp e\<cdot>u \<sqsubseteq> ae".
-    hence "ABinds (restrictA (edom ce) (delete x \<Gamma>))\<cdot>ae \<squnion> Aexp e\<cdot>u \<sqsubseteq> ae" by (simp add: restr_delete_twist)
+    from Abinds_reorder1[OF `map_of \<Gamma> x = Some e`] `ae x = up\<cdot>u`
+    have "ABinds (delete x \<Gamma>)\<cdot>ae \<squnion> Aexp e\<cdot>u = ABinds \<Gamma>\<cdot>ae" by (auto intro: join_comm)
+    moreover have "\<dots> f|` edom ce \<sqsubseteq> ae" using thunk by (auto simp add: join_below_iff env_restr_join)
+    ultimately have "(ABinds (delete x \<Gamma>)\<cdot>ae \<squnion> Aexp e\<cdot>u) f|` edom ce \<sqsubseteq> ae" by simp
 
     show ?case
     proof(cases "ce x" rule:two_cases)
@@ -166,28 +167,39 @@ begin
       have "(record_call x \<cdot> (prognosis ae a (\<Gamma>, Var x, S))) x = none"
         by (simp add: two_pred_none)
       hence **: "prognosis ae u (delete x \<Gamma>, e, Upd x # S) x = none" using fun_belowD[OF *, where x = x] by auto
-  
+
+      have eq: "prognosis (env_delete x ae) u (delete x \<Gamma>, e, Upd x # S) = prognosis ae u (delete x \<Gamma>, e, Upd x # S)"
+        by (rule prognosis_env_cong) simp
+
       have [simp]: "restr_stack (edom ce - {x}) S = restr_stack (edom ce) S" 
         using `x \<notin> upds S` by (auto intro: restr_stack_cong)
     
-      have "prognosis (ae) u (delete x \<Gamma>, e, Upd x # S) \<sqsubseteq> env_delete x ce"
+      have "prognosis (env_delete x ae) u (delete x \<Gamma>, e, Upd x # S) \<sqsubseteq> env_delete x ce"
+        unfolding eq
         using ** below_trans[OF below_trans[OF * Cfun.monofun_cfun_arg[OF `prognosis ae a (\<Gamma>, Var x, S) \<sqsubseteq> ce`]] record_call_below_arg]
         by (rule below_env_deleteI)
       moreover
-  
-      note `ABinds (restrictA (edom ce) (delete x \<Gamma>))\<cdot>ae \<squnion> Aexp e\<cdot>u \<sqsubseteq> ae`
+
+      have "ABinds (delete x \<Gamma>)\<cdot>(env_delete x ae) = ABinds (delete x \<Gamma>)\<cdot>ae" by (rule Abinds_env_cong) simp
+      with `(ABinds (delete x \<Gamma>)\<cdot>ae \<squnion> Aexp e\<cdot>u) f|\` edom ce \<sqsubseteq> ae`
+      have "(ABinds (delete x \<Gamma>)\<cdot>(env_delete x ae) \<squnion> Aexp e\<cdot>u) f|` edom ce \<sqsubseteq> ae" by simp
+      from env_restr_mono[where S = "-{x}", OF this]
+      have "(ABinds (delete x \<Gamma>)\<cdot>(env_delete x ae) \<squnion> Aexp e\<cdot>u) f|` edom (env_delete x ce) \<sqsubseteq> env_delete x ae"
+        by (auto simp add: Diff_eq Int_commute env_delete_restr)
+
       moreover
   
-      have "const_on ae (ap S) (up\<cdot>0)" using thunk by auto
-      hence "const_on ae (ap S) (up\<cdot>0)" using `x \<notin>  ap S`
-        by (fastforce simp add:  env_delete_def)
+      have "const_on ae (ap S \<inter> edom ce) (up\<cdot>0)" using thunk by auto
+      hence "const_on (env_delete x ae) (ap S \<inter> edom ce) (up\<cdot>0)" using `x \<notin>  ap S`
+        by (fastforce simp add: env_delete_def)
       moreover
   
-      have "const_on ae  (upds (restr_stack (edom ce) S)) (up\<cdot>0)" using thunk by auto
+      have "const_on ae (upds S \<inter> edom ce) (up\<cdot>0)" using thunk by auto
+      hence "const_on (env_delete x ae) (upds S \<inter> (edom (env_delete x ce))) (up\<cdot>0)" by fastforce
       ultimately
-      have "consistent (ae, env_delete x ce, u) (delete x \<Gamma>, e, Upd x # S)" using thunk `a \<sqsubseteq> u`
-        by (auto simp add: join_below_iff insert_absorb restr_delete_twist elim:below_trans)
-       
+
+      have "consistent (env_delete x ae, env_delete x ce, u) (delete x \<Gamma>, e, Upd x # S)" using thunk `a \<sqsubseteq> u`
+        by (auto simp add: join_below_iff env_restr_join insert_absorb restr_delete_twist elim:below_trans below_trans[OF env_restr_mono2, rotated])
       moreover
       
       {
@@ -204,10 +216,10 @@ begin
       have "\<dots> \<Rightarrow>\<^sub>G\<^sup>* (restrictA (edom ce)  (delete x (map_transform Aeta_expand ae (map_transform ccTransform ae \<Gamma>))), ccTransform u e, restr_stack (edom ce) S)"
         by (intro normal_trans Aeta_expand_correct `Astack (restr_stack (edom ce) S) \<sqsubseteq> u`)
       also(rtranclp_trans)
-      have "\<dots> = conf_transform (ae, env_delete x ce, u) (delete x \<Gamma>, e, Upd x # S)" 
+      have "\<dots> = conf_transform (env_delete x ae, env_delete x ce, u) (delete x \<Gamma>, e, Upd x # S)" 
         by (auto simp add:  map_transform_delete delete_map_transform_env_delete insert_absorb restr_delete_twist)
       finally(back_subst)
-      have "conf_transform (ae, ce, a) (\<Gamma>, Var x, S) \<Rightarrow>\<^sub>G\<^sup>* conf_transform (ae, env_delete x ce, u) (delete x \<Gamma>, e, Upd x # S)".
+      have "conf_transform (ae, ce, a) (\<Gamma>, Var x, S) \<Rightarrow>\<^sub>G\<^sup>* conf_transform (env_delete x ae, env_delete x ce, u) (delete x \<Gamma>, e, Upd x # S)".
       }
       ultimately
       show ?thesis by (blast del: consistentI consistentE)
@@ -228,7 +240,7 @@ begin
       
       have "prognosis ae 0 (delete x \<Gamma>, e, Upd x # S) \<sqsubseteq> ce" using *[unfolded `u=0`] thunk by (auto elim: below_trans)
       moreover
-      note `ABinds (restrictA (edom ce) (delete x \<Gamma>))\<cdot>ae \<squnion> Aexp e\<cdot>u \<sqsubseteq> ae`
+      note `(ABinds (delete x \<Gamma>)\<cdot>ae \<squnion> Aexp e\<cdot>u) f|\` edom ce \<sqsubseteq> ae`
       ultimately
       have "consistent (ae, ce, 0) (delete x \<Gamma>, e, Upd x # S)" using thunk `ae x = up\<cdot>u` `u = 0`  by auto
       moreover
@@ -244,26 +256,24 @@ begin
     qed
   next
   case (lamvar \<Gamma> x e S)
-    from lamvar have [simp]: "x \<in> domA \<Gamma>" by auto (metis domI dom_map_of_conv_domA)
-    from lamvar have "Aexp (Var x)\<cdot>a \<sqsubseteq> ae" by (auto simp add: join_below_iff)
-    from below_trans[OF Aexp_Var fun_belowD[OF this] ]
-    have "up\<cdot>a \<sqsubseteq> ae x".
-    then obtain u where "ae x = up\<cdot>u" and "a \<sqsubseteq> u" by (cases "ae x") auto
-    hence "x \<in> edom ae" by (auto simp add: edom_def)
-  
     from lamvar have "prognosis ae a (\<Gamma>, Var x, S) \<sqsubseteq> ce" by auto
     from below_trans[OF prognosis_called fun_belowD[OF this] ]
     have [simp]: "x \<in> edom ce" by (auto simp add: edom_def)
     then obtain c where "ce x = up\<cdot>c" by (cases "ce x") (auto simp add: edom_def)
 
-    from `map_of \<Gamma> x = Some e`
-    have "map_of (restrictA (edom ce) \<Gamma>) x = Some e" by simp
-    from Abinds_reorder1[OF this] `ae x = up\<cdot>u`
-    have "ABinds (delete x (restrictA (edom ce) \<Gamma>))\<cdot>ae \<squnion> Aexp e\<cdot>u = ABinds (restrictA (edom ce) \<Gamma>)\<cdot>ae" by (auto intro: join_comm)
-    also have "\<dots> \<sqsubseteq> ae" using lamvar by (auto simp add: join_below_iff)
-    finally have "ABinds (delete x (restrictA (edom ce) \<Gamma>))\<cdot>ae \<squnion> Aexp e\<cdot>u \<sqsubseteq> ae".
-    hence "ABinds (restrictA (edom ce) (delete x \<Gamma>))\<cdot>ae \<squnion> Aexp e\<cdot>u \<sqsubseteq> ae" by (simp add: restr_delete_twist)
+    from lamvar have [simp]: "x \<in> domA \<Gamma>" by auto (metis domI dom_map_of_conv_domA)
+    from lamvar have "Aexp (Var x)\<cdot>a f|` edom ce \<sqsubseteq> ae" by (auto simp add: join_below_iff env_restr_join)
+    from fun_belowD[where x = x, OF this] 
+    have "(Aexp (Var x)\<cdot>a) x \<sqsubseteq> ae x" by simp
+    from below_trans[OF Aexp_Var this]
+    have "up\<cdot>a \<sqsubseteq> ae x".
+    then obtain u where "ae x = up\<cdot>u" and "a \<sqsubseteq> u" by (cases "ae x") auto
+    hence "x \<in> edom ae" by (auto simp add: edom_def)
 
+    from Abinds_reorder1[OF `map_of \<Gamma> x = Some e`] `ae x = up\<cdot>u`
+    have "ABinds (delete x \<Gamma>)\<cdot>ae \<squnion> Aexp e\<cdot>u = ABinds \<Gamma>\<cdot>ae" by (auto intro: join_comm)
+    moreover have "\<dots> f|` edom ce \<sqsubseteq> ae" using lamvar by (auto simp add: join_below_iff env_restr_join)
+    ultimately have "(ABinds (delete x \<Gamma>)\<cdot>ae \<squnion> Aexp e\<cdot>u) f|` edom ce \<sqsubseteq> ae" by simp
 
     have "prognosis ae u ((x, e) # delete x \<Gamma>, e, S) = prognosis ae u (\<Gamma>, e, S)"
       using `map_of \<Gamma> x = Some e` by (auto intro!: prognosis_reorder)
@@ -273,8 +283,8 @@ begin
     finally have *: "prognosis ae u ((x, e) # delete x \<Gamma>, e, S) \<sqsubseteq> prognosis ae a (\<Gamma>, Var x, S)" by this simp_all
   
     have "consistent (ae, ce, u) ((x, e) # delete x \<Gamma>, e, S)"
-      using lamvar `ABinds (restrictA (edom ce) (delete x \<Gamma>))\<cdot>ae \<squnion> Aexp e\<cdot>u \<sqsubseteq> ae`  `ae x = up\<cdot>u` edom_mono[OF *]
-      by (auto simp add: join_below_iff thunks_Cons restr_delete_twist split:if_splits intro: below_trans[OF _ `a \<sqsubseteq> u`] below_trans[OF *])
+      using lamvar `(ABinds (delete x \<Gamma>)\<cdot>ae \<squnion> Aexp e\<cdot>u) f|\` edom ce \<sqsubseteq> ae`   `ae x = up\<cdot>u` edom_mono[OF *]
+      by (auto simp add: join_below_iff env_restr_join thunks_Cons restr_delete_twist split:if_splits intro: below_trans[OF _ `a \<sqsubseteq> u`] below_trans[OF *])
     moreover
   
     have "Astack (restr_stack (edom ce) S) \<sqsubseteq> u" using lamvar below_trans[OF _ `a \<sqsubseteq> u`] by auto
@@ -316,15 +326,9 @@ begin
       from `isLam e` `x \<notin> domA \<Gamma>`
       have *: "prognosis ae 0 ((x, e) # \<Gamma>, e, S) \<sqsubseteq> prognosis ae 0 (\<Gamma>, e, Upd x # S)" by (rule prognosis_Var2)
 
-      have "ABinds (restrictA (edom ce - {x}) \<Gamma>)\<cdot>ae = ABinds (delete x (restrictA (edom ce) \<Gamma>))\<cdot>ae" by simp
-      also have "\<dots> \<sqsubseteq> ABinds (restrictA (edom ce) \<Gamma>)\<cdot>ae"
-        by (rule ABinds_delete_below)
-      also have "ABinds (restrictA (edom ce) \<Gamma>)\<cdot>ae \<sqsubseteq> ae" using var\<^sub>2 by (auto simp add: join_below_iff)
-      finally have "ABinds (restrictA (edom ce - {x}) \<Gamma>)\<cdot>ae \<sqsubseteq> ae" by this simp
-  
       have "consistent (ae, ce, 0) ((x, e) # \<Gamma>, e, S)"
-        using var\<^sub>2 `ABinds (restrictA (edom ce - {x}) \<Gamma>)\<cdot>ae \<sqsubseteq> ae`
-        by (auto simp add: join_below_iff thunks_Cons split:if_splits elim:below_trans[OF *])
+        using var\<^sub>2
+        by (auto simp add: join_below_iff env_restr_join thunks_Cons split:if_splits elim:below_trans[OF *])
       moreover
       have "conf_transform (ae, ce, a) (\<Gamma>, e, Upd x # S) \<Rightarrow>\<^sub>G conf_transform (ae, ce, 0) ((x, e) # \<Gamma>, e, S)"
         using `ae x = up\<cdot>a` `a = 0` var\<^sub>2 `ce x = up\<cdot>c`
@@ -333,19 +337,23 @@ begin
     next
       case False[simp]
       hence "ce x = \<bottom>" using var\<^sub>2 by (auto simp add: edom_def)
+
+      from False have "x \<notin> edom ae" using var\<^sub>2 by auto
+      hence [simp]: "ae x = \<bottom>" by (auto simp add: edom_def)
+
       
       have "prognosis ae a ((x, e) # \<Gamma>, e, S) \<sqsubseteq> prognosis ae a ((x, e) # \<Gamma>, e, Upd x # S)" by (rule prognosis_upd)
       also
-
-      from `ce x = \<bottom>` and var\<^sub>2
-      have "prognosis ae a (\<Gamma>, e, Upd x # S) x = \<bottom>" by auto (metis below_bottom_iff fun_belowD)
-      hence "prognosis ae a ((x, e) # \<Gamma>, e, Upd x # S) = prognosis ae a (\<Gamma>, e, Upd x # S)" using `x \<notin> domA \<Gamma>`
+       
+      from `ae x = \<bottom>`
+      have "prognosis ae a ((x, e) # \<Gamma>, e, Upd x # S) \<sqsubseteq> prognosis ae a (delete x ((x,e) # \<Gamma>), e, Upd x # S)"
         by (rule prognosis_not_called)
+      also have  "delete x ((x,e)#\<Gamma>) = \<Gamma>" using `x \<notin> domA \<Gamma>` by simp
       finally
-      have *: "prognosis ae a ((x, e) # \<Gamma>, e, S) \<sqsubseteq> prognosis ae a (\<Gamma>, e, Upd x # S)".
-  
+      have *: "prognosis ae a ((x, e) # \<Gamma>, e, S) \<sqsubseteq> prognosis ae a (\<Gamma>, e, Upd x # S)" by this simp
+
       have "consistent (ae, ce, a) ((x, e) # \<Gamma>, e, S)" using var\<^sub>2
-        by (auto simp add: join_below_iff `ce x = \<bottom>` thunks_Cons split:if_splits elim:below_trans[OF *])
+        by (auto simp add: join_below_iff env_restr_join `ce x = \<bottom>` thunks_Cons split:if_splits elim:below_trans[OF *])
       moreover
       have "conf_transform (ae, ce, a) (\<Gamma>, e, Upd x # S) = conf_transform (ae, ce, a) ((x, e) # \<Gamma>, e, S)"
         by(simp add: map_transform_restrA[symmetric])
@@ -387,11 +395,11 @@ begin
     have [simp]: "\<And> S. S \<subseteq> domA \<Gamma> \<Longrightarrow> ?ae f|` S = \<bottom>" by (auto dest!: set_mp[OF edom_Aheap])
   
     {
-    have "edom (?ae \<squnion> ae) \<subseteq> domA (\<Delta> @ \<Gamma>) \<union> upds S"
-      using let\<^sub>1(3) by (auto dest: set_mp[OF edom_Aheap])
-    moreover
     have "edom (?ce \<squnion> ce) \<subseteq> domA (\<Delta> @ \<Gamma>) \<union> upds S"
       using let\<^sub>1(3) by (auto simp add: edom_cHeap dest: set_mp[OF edom_Aheap])
+    moreover
+    have "edom (?ae \<squnion> ae) = edom (?ce \<squnion> ce)"
+      using let\<^sub>1(3) by (auto simp add: edom_cHeap)
     moreover
     { fix x e'
       assume "x \<in> thunks \<Gamma>"
@@ -416,8 +424,13 @@ begin
       have "(?ae \<squnion> ae) x = up\<cdot>0" by (auto simp add: Aheap_heap3)
     }
     moreover
-    have "const_on ae (ap S) (up\<cdot>0)" using let\<^sub>1 by auto  
-    hence "const_on (?ae \<squnion> ae) (ap S) (up\<cdot>0)" by fastforce
+    have [simp]: "ap S \<inter> edom (cHeap \<Delta> e\<cdot>a) = {}"
+      using fresh_distinct_fv[OF let\<^sub>1(2)] 
+      by (auto simp add: edom_cHeap dest!: set_mp[OF edom_Aheap] set_mp[OF ap_fv_subset])
+
+    have "const_on ae (ap S \<inter> edom ce) (up\<cdot>0)" using let\<^sub>1 by auto  
+    hence "const_on (?ae \<squnion> ae) (ap S \<inter> edom ce) (up\<cdot>0)" by fastforce
+    hence "const_on (?ae \<squnion> ae) (ap S \<inter> edom (?ce \<squnion> ce)) (up\<cdot>0)" by (simp add: Int_Un_distrib)
     moreover
     have "const_on ae (upds (restr_stack (edom ce) S)) (up\<cdot>0)" using let\<^sub>1 by auto
     hence "const_on (?ae \<squnion> ae) (upds (restr_stack (edom ce) S)) (up\<cdot>0)"  by fastforce
@@ -439,33 +452,30 @@ begin
     have "heap_upds_ok (\<Delta> @ \<Gamma>, S)" by (rule heap_upds_ok_append)
     moreover
     {
-    from  fresh_distinct[OF let\<^sub>1(1)]
-    have  disj: "domA (restrictA (edom ?ce) \<Delta>) \<inter> domA (restrictA (edom ce) \<Gamma>) = {}" by auto
-
-    have re1: "restrictA (edom (?ce \<squnion> ce)) \<Delta> = restrictA (edom ?ce) \<Delta>"
-      using `edom ce \<inter> domA \<Delta> = {}` by (auto intro: restrictA_cong)
-    moreover
-    have re2: "restrictA (edom (?ce \<squnion> ce)) \<Gamma> = restrictA (edom ce) \<Gamma>"
-      using `edom ?ce \<inter> domA \<Gamma> = {}` by (auto intro: restrictA_cong)
-    moreover
-    have "ABinds (restrictA (edom ?ce) \<Delta>)\<cdot>(Aheap \<Delta> e\<cdot>a \<squnion> ae) = ABinds (restrictA (edom ?ce) \<Delta>)\<cdot>(Aheap \<Delta> e\<cdot>a)"
+    have "ABinds \<Delta>\<cdot>(Aheap \<Delta> e\<cdot>a \<squnion> ae) = ABinds \<Delta>\<cdot>(Aheap \<Delta> e\<cdot>a)"
       by (rule Abinds_env_restr_cong) (simp add: env_restr_join)
     moreover
-    have "ABinds (restrictA (edom ce) \<Gamma>)\<cdot>(Aheap \<Delta> e\<cdot>a \<squnion> ae) = ABinds (restrictA (edom ce) \<Gamma>)\<cdot>ae"
+    have "ABinds \<Gamma>\<cdot>(Aheap \<Delta> e\<cdot>a \<squnion> ae) = ABinds \<Gamma>\<cdot>ae"
       by (rule Abinds_env_restr_cong) (simp add: env_restr_join)
-    moreover
-    have "ABinds (restrictA (edom ?ce) \<Delta>)\<cdot>(Aheap \<Delta> e\<cdot>a) \<sqsubseteq> ABinds \<Delta>\<cdot>(Aheap \<Delta> e\<cdot>a)"
-      by (rule ABinds_restrict_below)
     moreover
     have "ABinds \<Delta>\<cdot>(Aheap \<Delta> e\<cdot>a) \<squnion> Aexp e\<cdot>a \<sqsubseteq> Aheap \<Delta> e\<cdot>a \<squnion> Aexp (Let \<Delta> e)\<cdot>a" by (rule Aexp_Let)
-    moreover have " ABinds (restrictA (edom ce) \<Gamma>)\<cdot>ae \<squnion> Aexp (Let \<Delta> e)\<cdot>a \<sqsubseteq> ae" using let\<^sub>1 by auto
+    moreover
+    have "(ABinds \<Gamma>\<cdot>ae \<squnion> Aexp (Let \<Delta> e)\<cdot>a) f|` edom ce \<sqsubseteq> ae" using let\<^sub>1 by auto
+    moreover
+    have "Aexp (Terms.Let \<Delta> e)\<cdot>a f|` (edom ce \<union> edom (cHeap \<Delta> e\<cdot>a)) = Aexp (Terms.Let \<Delta> e)\<cdot>a f|` edom ce"
+      by (rule env_restr_cong) (auto simp add: edom_cHeap dest!: set_mp[OF Aexp_edom]  set_mp[OF edom_Aheap])
+    moreover
+    have "ABinds \<Gamma>\<cdot>ae f|` (edom ce \<union> edom (cHeap \<Delta> e\<cdot>a)) = ABinds \<Gamma>\<cdot>ae f|` edom ce" 
+      using fresh_distinct_fv[OF let\<^sub>1(1)]
+      by (auto intro: env_restr_cong  simp add: edom_cHeap dest!: set_mp[OF Aexp_edom]  set_mp[OF edom_Aheap] set_mp[OF edom_AnalBinds])
     ultimately
-    have "ABinds (restrictA (edom (?ce \<squnion> ce)) (\<Delta> @ \<Gamma>)) \<cdot> (Aheap \<Delta> e\<cdot>a \<squnion> ae) \<squnion> Aexp e\<cdot>a \<sqsubseteq> Aheap \<Delta> e\<cdot>a \<squnion> ae"
-      by (simp only: join_assoc[symmetric] restrictA_append Abinds_append_disjoint[OF disj] join_below_iff)
-         (auto simp add: join_below_iff elim!: below_trans)
+    have "(ABinds (\<Delta> @ \<Gamma>) \<cdot> (Aheap \<Delta> e\<cdot>a \<squnion> ae) \<squnion> Aexp e\<cdot>a) f|` edom (?ce \<squnion> ce) \<sqsubseteq> Aheap \<Delta> e\<cdot>a \<squnion> ae"
+      by (simp only: join_assoc[symmetric] restrictA_append Abinds_append_disjoint[OF fresh_distinct[OF let\<^sub>1(1)]] join_below_iff env_restr_join)
+         (auto 4 4 simp add: join_below_iff env_restr_join intro: below_trans[OF env_restr_below_self] elim!: below_trans[OF env_restr_mono] below_trans)
     }
     ultimately
-    have "consistent (?ae \<squnion> ae, ?ce \<squnion> ce, a) (\<Delta> @ \<Gamma>, e, S) " by auto
+    have "consistent (?ae \<squnion> ae, ?ce \<squnion> ce, a) (\<Delta> @ \<Gamma>, e, S) "
+      by auto
     }
     moreover
     {
