ROOT
@@ -45,6 +45,7 @@ session Arity (AFP) in "Launchbury" = "HOLCF-Nominal2" +
     "NoCardinalityAnalysis"
     "FTreeCardinality"
     "CoCallImplCorrect"
+    "CallArityCorrectEnd2End"
 
 session Nominal2013_1 in "Nominal2-Isabelle2013-1/Nominal" = HOL +
   theories
